fairness/model_plug.v
@@ -1,5 +1,6 @@
 From trillium.fairness Require Import resources execution_model fairness. 
 From iris.base_logic.lib Require Import invariants.
+From iris.proofmode Require Import tactics.
 
 Section ModelPlug.
   (* Context `{Countable G}.  *)
@@ -14,11 +15,14 @@ Section ModelPlug.
   (* Context {PMPP: @PartialModelPredicatesPre G _ _ Σ iM}. *)
 
   Context (relies_on: locale Λ -> fmrole M -> iProp Σ).
-  Context (ε: coPset). 
+  Context (ε: coPset).
+
+  (* Definition model_lifted_step (P Q: iProp Σ) *)
+  (*   (τ: locale Λ) (extr: execution_trace Λ) (auxtr: auxiliary_trace M__glob) c2 *)
 
   Definition model_plugged: iProp Σ :=
     ∀ P Q (gl: fmrole M),
-      □ (∀ (δ: fmstate M), P ∗ msi δ ==∗ ∃ δ', Q ∗ msi δ' ∗ ⌜ fmtrans M δ (Some gl) δ' ⌝) →
+       □ ((∀ (δ: fmstate M), P ∗ msi δ ==∗ ∃ δ', Q ∗ msi δ' ∗ ⌜ fmtrans M δ (Some gl) δ' ⌝) →
       (∀ (τ: locale Λ) (extr: execution_trace Λ) (auxtr: auxiliary_trace M__glob) c2,
         relies_on τ gl ∗
         P ∗ 
@@ -29,6 +33,6 @@ Section ModelPlug.
          relies_on τ gl ∗
          Q ∗
          em_msi c2 δ2 (em_GS0 := eGS) ∗
-         ⌜em_valid_state_evolution_fairness (extr :tr[ Some τ ]: c2) (auxtr :tr[ ℓ ]: δ2)⌝).
+         ⌜em_valid_state_evolution_fairness (extr :tr[ Some τ ]: c2) (auxtr :tr[ ℓ ]: δ2)⌝)).
 
 End ModelPlug.
